证明：

### **$n=k$时**

$$
\beta \left( {\sum\limits_{i = 1}^k {\sum\limits_{i = 1}^k {{q_i}} } } \right) + n\left( {\sum\limits_{i = 1}^k {\left( { - \beta n{q_i} + \beta \left( {\sum\limits_{i = 1}^k {{q_i}} } \right) - {q_i}} \right)} } \right) + \left( {1 - \beta } \right)\left( {\sum\limits_{i = 1}^k {{q_i}} } \right)=0
$$

化简得
$$
\beta k\sum\limits_{i = 1}^k {{q_i}}  + n\left( { - \beta n\sum\limits_{i = 1}^k {{q_i}}  + \beta k\sum\limits_{i = 1}^k {{q_i}}  - \sum\limits_{i = 1}^k {{q_i}} } \right) + \left( {1 - \beta } \right)\left( {\sum\limits_{i = 1}^k {{q_i}} } \right)=0
$$
得
$$
\beta k\sum\limits_{i = 1}^k {{q_i}}  - \beta {n^2}\sum\limits_{i = 1}^k {{q_i}}  + n\beta k\sum\limits_{i = 1}^k {{q_i}}  - n\sum\limits_{i = 1}^k {{q_i}}  + \left( {1 - \beta } \right)\left( {\sum\limits_{i = 1}^k {{q_i}} } \right)=0
$$
合并$\sum\limits_{i = 1}^k {{q_i}} $，得
$$
\left( {\beta k - \beta {n^2} + n\beta k - n + \left( {1 - \beta } \right)} \right)\sum\limits_{i = 1}^k {{q_i}}=0
$$
化简并代入$n=k$得
$$
\left( {k - 1} \right)\left( {\beta  - 1} \right)\sum\limits_{i = 1}^k {{q_i}} =0
$$

得$\beta=1$

### **$n=k+1$时**

$$
\beta \left( {\sum\limits_{i = 1}^{k + 1} {\sum\limits_{i = 1}^{k + 1} {{q_i}} } } \right) + n\left( {\sum\limits_{i = 1}^{k + 1} {\left( { - \beta n{q_i} + \beta \left( {\sum\limits_{i = 1}^{k + 1} {{q_i}} } \right) - {q_i}} \right)} } \right) + \left( {1 - \beta } \right)\left( {\sum\limits_{i = 1}^{k + 1} {{q_i}} } \right)
$$

化简得
$$
\beta \left( {k + 1} \right)\sum\limits_{i = 1}^{k + 1} {{q_i}}  - \beta {n^2}\sum\limits_{i = 1}^{k + 1} {{q_i}}  + n\beta \left( {k + 1} \right)\sum\limits_{i = 1}^{k + 1} {{q_i}}  - n\sum\limits_{i = 1}^{k + 1} {{q_i}}  + \left( {1 - \beta } \right)\left( {\sum\limits_{i = 1}^{k+1} {{q_i}} } \right)
$$
合并$\sum\limits_{i = 1}^{k+1} {{q_i}} $，得
$$
\left( {\beta \left( {k + 1} \right) - \beta {n^2} + n\beta \left( {k + 1} \right) - n + \left( {1 - \beta } \right)} \right)\sum\limits_{i = 1}^{k + 1} {{q_i}}
$$
代入$n=k+1$得
$$
k\left( {\beta  - 1} \right)\sum\limits_{i = 1}^{k+1} {{q_i}}=0
$$

$$
\left( {\sum\limits_{i = 1}^n {\left( {\sum\limits_{i = 1}^n {{q_i}} } \right)} {q_i}} \right) = \sum\limits_{i = 1}^n {\sum\limits_{j = 1}^n {{q_i}{q_j}} }  = \left( {\sum\limits_{i = 1}^n {{q_i}} } \right)\left( {\sum\limits_{i = 1}^n {{q_i}} } \right)
$$

$$
\left( {\sum\limits_{i = 1}^n {\left( {\sum\limits_{i = 1}^n {{q_i}} } \right)} {q_i}} \right) = {\left( {\sum\limits_{i = 1}^n {{q_i}} } \right)^2}
$$

$$
\sum\limits_{i = 1}^n {q_i^2}  + \sum\limits_{i,j,i \ne j}^n {{q_i}{q_j}} 
$$

